cedar-lean/Cedar/Thm/Validation/Levels.lean
@@ -37,7 +37,7 @@ open Cedar.Data
 open Cedar.Spec
 open Cedar.Validation
 
-theorem level_based_slicing_is_sound {e : Expr} {n : Nat} {tx : TypedExpr} {c c₁ : Capabilities} {env : Environment} {request : Request} {entities slice : Entities}
+theorem level_based_slicing_is_sound_expr {e : Expr} {n : Nat} {tx : TypedExpr} {c c₁ : Capabilities} {env : Environment} {request : Request} {entities slice : Entities}
   (hs : slice = entities.sliceAtLevel request n)
   (hc : CapabilitiesInvariant c request entities)
   (hr : RequestAndEntitiesMatchEnvironment env request entities)
@@ -49,30 +49,30 @@ theorem level_based_slicing_is_sound {e : Expr} {n : Nat} {tx : TypedExpr} {c c�
   case lit => simp [evaluate]
   case var v => cases v <;> simp [evaluate]
   case ite c t e =>
-    have ihc := @level_based_slicing_is_sound c
-    have iht := @level_based_slicing_is_sound t
-    have ihe := @level_based_slicing_is_sound e
+    have ihc := @level_based_slicing_is_sound_expr c
+    have iht := @level_based_slicing_is_sound_expr t
+    have ihe := @level_based_slicing_is_sound_expr e
     exact level_based_slicing_is_sound_if hs hc hr ht hl ihc iht ihe
   case and e₁ e₂ =>
-    have ih₁ := @level_based_slicing_is_sound e₁
-    have ih₂ := @level_based_slicing_is_sound e₂
+    have ih₁ := @level_based_slicing_is_sound_expr e₁
+    have ih₂ := @level_based_slicing_is_sound_expr e₂
     exact level_based_slicing_is_sound_and hs hc hr ht hl ih₁ ih₂
   case or e₁ e₂ =>
-    have ih₁ := @level_based_slicing_is_sound e₁
-    have ih₂ := @level_based_slicing_is_sound e₂
+    have ih₁ := @level_based_slicing_is_sound_expr e₁
+    have ih₂ := @level_based_slicing_is_sound_expr e₂
     exact level_based_slicing_is_sound_or hs hc hr ht hl ih₁ ih₂
   case unaryApp op e =>
-    have ihe := @level_based_slicing_is_sound e
+    have ihe := @level_based_slicing_is_sound_expr e
     exact level_based_slicing_is_sound_unary_app hs hc hr ht hl ihe
   case binaryApp op e₁ e₂ =>
-    have ihe₁ := @level_based_slicing_is_sound e₁
-    have ihe₂ := @level_based_slicing_is_sound e₂
+    have ihe₁ := @level_based_slicing_is_sound_expr e₁
+    have ihe₂ := @level_based_slicing_is_sound_expr e₂
     exact level_based_slicing_is_sound_binary_app hs hc hr ht hl ihe₁ ihe₂
   case getAttr e _ =>
-    have ihe := @level_based_slicing_is_sound e
+    have ihe := @level_based_slicing_is_sound_expr e
     exact level_based_slicing_is_sound_get_attr hs hc hr ht hl ihe
   case hasAttr e _ =>
-    have ihe := @level_based_slicing_is_sound e
+    have ihe := @level_based_slicing_is_sound_expr e
     exact level_based_slicing_is_sound_has_attr hs hc hr ht hl ihe
   case set => sorry -- trivial recursive case maybe a little tricky
   case call => sorry -- should be the same as set
@@ -84,6 +84,21 @@ theorem level_based_slicing_is_sound {e : Expr} {n : Nat} {tx : TypedExpr} {c c�
         rw [Prod.mk.sizeOf_spec] at h₁
         simp only [Expr.record.sizeOf_spec]
         omega
-      exact @level_based_slicing_is_sound x.snd
+      exact @level_based_slicing_is_sound_expr x.snd
     exact level_based_slicing_is_sound_record hs hc hr ht hl ih
 termination_by e
+
+theorem level_based_slicing_is_sound {p : Policy} {n : Nat} {env : Environment} {request : Request} {entities slice : Entities}
+  (hs : slice = entities.sliceAtLevel request n)
+  (hr : RequestAndEntitiesMatchEnvironment env request entities)
+  (htl : typecheckAtLevel p env n = true) :
+  evaluate p.toExpr request entities = evaluate p.toExpr request slice
+:= by
+  simp only [typecheckAtLevel] at htl
+  cases ht : typeOf p.toExpr ∅ env <;> (
+    rw [ht] at htl
+    simp only [Bool.false_eq_true] at htl
+  )
+  rw [←level_spec] at htl
+  have hc := empty_capabilities_invariant request entities
+  exact level_based_slicing_is_sound_expr hs hc hr ht htl
